formula_prices_list.thy
@@ -11,61 +11,7 @@ expr_1_tt: \<open>expr_1 TT = 0\<close> |
 expr_1_conj: \<open>expr_1 (hml_conj I J \<Phi>) = Sup ((expr_1 \<circ> \<Phi>) ` I \<union> (expr_1 \<circ> \<Phi>) ` J)\<close> |
 expr_1_pos: \<open>expr_1 (hml_pos \<alpha> \<phi>) = 
   1 + (expr_1 \<phi>)\<close>
-(*
-(*Done*)
-lemma expr_1_set_form: "expr_1 (HML_conj \<Phi> \<Psi>) =
-Max({0} \<union> {expr_1 x | x. x \<in> set \<Phi>} \<union> {expr_1 y | y. y \<in> set \<Psi>})"
-  apply((cases \<Phi>), (cases \<Psi>))
-proof-
-  assume assms: "\<Phi> = []" "\<Psi> = []"
-  hence "((expr_1 ` (set \<Phi>)) \<union> (expr_1 ` (set \<Psi>))) = {}"
-    by blast
-  hence e1_eq_0: "expr_1 (HML_conj \<Phi> \<Psi>) = 0"
-    using Sup_enat_def expr_1.simps(1)
-    by force
-  from assms have "({0} \<union> {expr_1 x | x. x \<in> set \<Phi>} \<union> {expr_1 y | y. y \<in> set \<Psi>}) = {0}"
-    by simp
-  hence "Max ({0} \<union> {expr_1 x | x. x \<in> set \<Phi>} \<union> {expr_1 y | y. y \<in> set \<Psi>}) = 0"
-    using Max_singleton
-    by metis
-  with e1_eq_0 show ?thesis
-    by presburger
-next
-  fix a tail
-  assume assms: "\<Phi> = []" "\<Psi> = a # tail"
-  have eq: "((expr_1 ` (set \<Phi>)) \<union> (expr_1 ` (set \<Psi>))) = ({expr_1 x | x. x \<in> set \<Phi>} \<union> {expr_1 y | y. y \<in> set \<Psi>})"
-    by blast
-  have fin_\<Psi>: "finite (set \<Psi>)"
-    by auto
-  from assms(2) have ne_\<Psi>: "(set \<Psi>) \<noteq> {}"
-    by simp
-  with assms(1) fin_\<Psi> have max_insert_0: "Max ({expr_1 x | x. x \<in> set \<Phi>} \<union> {expr_1 y | y. y \<in> set \<Psi>}) = 
-Max({0} \<union> {expr_1 x | x. x \<in> set \<Phi>} \<union> {expr_1 y | y. y \<in> set \<Psi>})"
-    using Max_insert
-    by auto
-  from assms fin_\<Psi> ne_\<Psi> Sup_enat_def have "expr_1 (HML_conj \<Phi> \<Psi>) = Max ((expr_1 ` (set \<Phi>)) \<union> (expr_1 ` (set \<Psi>)))"
-    by auto
-  with eq max_insert_0 show ?thesis using expr_1.simps(1)
-    by presburger
-next
-  fix a tail
-  assume \<Phi>_eq: "\<Phi> = a # tail"
-  have eq: "((expr_1 ` (set \<Phi>)) \<union> (expr_1 ` (set \<Psi>))) = ({expr_1 x | x. x \<in> set \<Phi>} \<union> {expr_1 y | y. y \<in> set \<Psi>})"
-    by blast
-  have fin_\<Phi>: "finite (set \<Phi>)"
-    by auto
-  from \<Phi>_eq have ne_\<Phi>: "(set \<Phi>) \<noteq> {}"
-    by simp
-  with fin_\<Phi> have max_insert_0: "Max ({expr_1 x | x. x \<in> set \<Phi>} \<union> {expr_1 y | y. y \<in> set \<Psi>}) = 
-Max({0} \<union> {expr_1 x | x. x \<in> set \<Phi>} \<union> {expr_1 y | y. y \<in> set \<Psi>})"
-    using Max_insert
-    by auto
-  from  fin_\<Phi> ne_\<Phi> Sup_enat_def have "expr_1 (HML_conj \<Phi> \<Psi>) = Max ((expr_1 ` (set \<Phi>)) \<union> (expr_1 ` (set \<Psi>)))"
-    by auto
-  with eq max_insert_0 show ?thesis using expr_1.simps(1)
-    by presburger
-qed
-*)
+
 
 primrec expr_2 :: "('a, 's)hml \<Rightarrow> enat"
   where
@@ -73,34 +19,12 @@ expr_2_tt: \<open>expr_2 TT = 1\<close> |
 expr_2_conj: \<open>expr_2 (hml_conj I J \<Phi>) = 1 + Sup ((expr_2 \<circ> \<Phi>) ` I \<union> (expr_2 \<circ> \<Phi>) ` J)\<close> |
 expr_2_pos: \<open>expr_2 (hml_pos \<alpha> \<phi>) = expr_2 \<phi>\<close>
 
-(*
-(*TODO*)
-lemma expr_2_set: "expr_2 (HML_conj \<Phi> \<Psi>) =
-Max({1} \<union> {1 + expr_2 x | x. x \<in> set \<Phi>} \<union> {1 + expr_2 y | y. y \<in> set \<Psi>})"
-  sorry
-*)
-
-(*
-fun r :: "('a, 's)hml set \<Rightarrow> enat"
-  where
-\<open>r xs = Max (set (map(\<lambda>x. expr_1 x) xs))\<close>
-*)
-
 
 primrec expr_3 :: "('a, 's) hml \<Rightarrow> enat"
   where
 expr_3_tt: \<open>expr_3 TT = 0\<close> |
  expr_3_pos: \<open>expr_3 (hml_pos \<alpha> \<phi>) = expr_3 \<phi>\<close> | 
 expr_3_conj: \<open>expr_3 (hml_conj I J \<Phi>) = (Sup ((expr_1 \<circ> \<Phi>) ` I \<union> (expr_3 \<circ> \<Phi>) ` I \<union> (expr_3 \<circ> \<Phi>) ` J))\<close>
-
-(*
-(*TODO*)
-lemma expr_3_set: "expr_3 (HML_conj \<Phi> \<Psi>) =
-Max({0} \<union> {expr_3 x | x. x \<in> set \<Phi>} \<union> {expr_3 y | y. y \<in> set \<Psi>} \<union> {expr_1 x | x. x \<in> set \<Phi>})"
-  sorry
-*)
-
-(* Neg := {i \<in> I| \<exists>\<phi>\<^sub>i. \<psi>\<^sub>i = \<not>\<phi>\<^sub>i}*)
 
 fun pos_r :: "('a, 's)hml set \<Rightarrow> ('a, 's)hml set"
   where
@@ -116,27 +40,12 @@ expr_4_tt: "expr_4 TT = 0" |
 expr_4_pos: "expr_4 (hml_pos a \<phi>) = expr_4 \<phi>" |
 expr_4_conj: "expr_4 (hml_conj I J \<Phi>) = Sup ((expr_1 ` (pos_r (\<Phi> ` I)))  \<union> (expr_4 \<circ> \<Phi>) ` I \<union> (expr_4 \<circ> \<Phi>) ` J)"
 
-(*
-(*Done*)
-lemma expr_4_set: "expr_4 (HML_conj \<Phi> \<Psi>) =
-Max ({expr_1 (HML_conj (pos_r \<Phi>)[])} \<union> {expr_4 x|x. x \<in> set \<Phi>} \<union> {expr_4 y|y. y \<in> set \<Psi>})"
-  sorry
-*)
-
 primrec expr_5 :: "('a, 's)hml \<Rightarrow> enat"
   where
 expr_5_tt: \<open>expr_5 TT = 0\<close> |
 expr_5_pos:\<open>expr_5 (hml_pos \<alpha> \<phi>) = expr_5 \<phi>\<close>|
 expr_5_conj: \<open>expr_5 (hml_conj I J \<Phi>) = 
 (Sup ((expr_5 \<circ> \<Phi>) ` I \<union> (expr_5 \<circ> \<Phi>) ` J \<union> (expr_1 \<circ> \<Phi>) ` J))\<close>
-
-(*
-lemma expr_5_set: "expr_5 (HML_conj \<Phi> \<Psi>) = 
-Max({0} \<union> {expr_5 x | x. x \<in> set \<Phi>} \<union> {expr_5 y | y. y \<in> set \<Psi>} \<union> {expr_1 y | y. y \<in> set \<Psi>})"
-  sorry
-*)
-
-find_theorems "enat" "Suc"
 
 primrec expr_6 :: "('a, 's)hml \<Rightarrow> enat"
   where
@@ -145,18 +54,9 @@ expr_6_pos: \<open>expr_6 (hml_pos \<alpha> \<phi>) = expr_6 \<phi>\<close>|
 expr_6_conj: \<open>expr_6 (hml_conj I J \<Phi>) = 
 (Sup ((expr_6 \<circ> \<Phi>) ` I \<union> ((eSuc \<circ> expr_6 \<circ> \<Phi>) ` J)))\<close>
 
-(*
-(*TODO*)
-lemma expr_6_set: "expr_6 (HML_conj \<Phi> \<Psi>) = 
-Max({0} \<union> {expr_6 x | x. x \<in> set \<Phi>} \<union> {1 + expr_6 y | y. y \<in> set \<Psi>})"
-  sorry
-*)
 
 fun expr :: "('a, 's)hml \<Rightarrow> enat \<times> enat \<times> enat \<times>  enat \<times> enat \<times> enat" 
   where
 \<open>expr \<phi> = (expr_1 \<phi>, expr_2 \<phi>, expr_3 \<phi>, expr_4 \<phi>, expr_5 \<phi>, expr_6 \<phi>)\<close>
                                  
-find_theorems expr
-thm Sup
-thm Max_def
 end
