HML_definitions.thy
@@ -1,0 +1,410 @@
+theory HML_definitions
+imports HML_list
+begin
+
+inductive hml_trace :: "('a, 's)hml \<Rightarrow> bool" where
+"hml_trace TT" |
+"hml_trace (hml_pos \<alpha> \<phi>)" if "hml_trace \<phi>"
+
+inductive hml_failure_trace :: "('a, 's)hml \<Rightarrow> bool" where
+"hml_failure_trace TT" |
+"hml_failure_trace (hml_pos \<alpha> \<phi>)" if "hml_failure_trace \<phi>" |
+"hml_failure_trace (hml_conj I J \<Phi>)" 
+  if "(\<Phi> ` I) = {} \<or> (\<exists>i \<in> \<Phi> ` I. \<Phi> ` I = {i} \<and> hml_failure_trace i)"
+     "\<forall>j \<in> \<Phi> ` J. \<exists>\<alpha>. j = (hml_pos \<alpha> TT) \<or> j = TT" 
+
+
+context lts begin 
+
+lemma 
+  fixes \<phi> :: "('a, 's) hml"
+  assumes "hml_trace \<phi>"
+  shows "\<exists>\<psi>. HML_trace \<psi> \<and> (\<forall>s. (s \<Turnstile> \<phi>) \<longleftrightarrow> (s \<Turnstile> \<psi>))"
+  using assms  
+proof(induction \<phi> rule: hml_trace.induct)
+  case 1
+  then show ?case using trace_tt by blast
+next
+  case (2 \<phi> \<alpha>)
+then obtain \<psi> where "HML_trace \<psi>" and IH: "(\<forall>s. (s \<Turnstile> \<phi>) = (s \<Turnstile> \<psi>))" by blast
+  hence "HML_trace (hml_pos \<alpha> \<psi>)" 
+    by (simp add: trace_pos)
+  have "(\<forall>s. (s \<Turnstile> hml_pos \<alpha> \<phi>) = (s \<Turnstile> (hml_pos \<alpha> \<psi>)))" using IH 
+    by simp
+  then show ?case 
+    using \<open>HML_trace (hml_pos \<alpha> \<psi>)\<close> by blast
+qed
+
+lemma 
+  fixes \<phi> :: "('a, 's) hml"
+  assumes "HML_trace \<phi>"
+  shows "\<exists>\<psi>. hml_trace \<psi> \<and> (\<forall>s. (s \<Turnstile> \<phi>) \<longleftrightarrow> (s \<Turnstile> \<psi>))"
+  using assms proof(induct)
+  case trace_tt
+  then show ?case 
+    using hml_trace.intros(1) by blast
+next
+  case (trace_conj \<psi>s)
+  have "hml_trace TT" 
+    using hml_trace.intros(1) by blast
+  have "(\<forall>s. (s \<Turnstile> hml_conj {} {} \<psi>s) = (s \<Turnstile> TT))" 
+    by simp
+  then show ?case using \<open>hml_trace TT\<close> by blast
+next
+  case (trace_pos \<phi> \<alpha>)
+  then obtain \<psi> where IH: "hml_trace \<psi>" "(\<forall>s. (s \<Turnstile> \<phi>) = (s \<Turnstile> \<psi>))" by blast
+  hence "(\<forall>s. (s \<Turnstile> hml_pos \<alpha> \<phi>) = (s \<Turnstile> (hml_pos \<alpha> \<psi>)))" using hml_sem_pos by simp
+  from IH have "hml_trace (hml_pos \<alpha> \<psi>)" 
+    using hml_trace.simps by blast
+  then show ?case using \<open>(\<forall>s. (s \<Turnstile> hml_pos \<alpha> \<phi>) = (s \<Turnstile> (hml_pos \<alpha> \<psi>)))\<close> 
+    by blast
+qed
+
+lemma 
+  fixes \<phi> :: "('a, 's) hml"
+  assumes "hml_failure_trace \<phi>"
+  shows "\<exists>\<psi>. HML_failure_trace \<psi> \<and> (\<forall>s. (s \<Turnstile> \<phi>) \<longleftrightarrow> (s \<Turnstile> \<psi>))"
+  using assms proof induct
+  case 1
+  then show ?case
+    using f_trace_tt by blast
+next
+  case (2 \<phi> \<alpha>)
+  then obtain \<psi> where "HML_failure_trace \<psi>" "(\<forall>s. (s \<Turnstile> \<phi>) = (s \<Turnstile> \<psi>))" by blast
+  have "HML_failure_trace (hml_pos \<alpha> \<psi>)" 
+    by (simp add: \<open>HML_failure_trace \<psi>\<close> f_trace_pos)
+  have "(\<forall>s. (s \<Turnstile> hml_pos \<alpha> \<phi>) = (s \<Turnstile> (hml_pos \<alpha> \<psi>)))" 
+    by (simp add: \<open>\<forall>s. (s \<Turnstile> \<phi>) = (s \<Turnstile> \<psi>)\<close>)
+  then show ?case 
+    using \<open>HML_failure_trace (hml_pos \<alpha> \<psi>)\<close> by blast
+next
+  case (3 \<Phi> I J)
+  hence neg_case: "\<forall>j\<in>\<Phi> ` J. stacked_pos_conj_pos j" 
+    using stacked_pos_conj_pos.simps nested_empty_pos_conj.intros(1) by auto
+  from 3(1) show ?case proof(rule disjE)
+    assume "\<Phi> ` I = {}"
+    hence "HML_failure_trace (hml_conj I J \<Phi>) \<and> (\<forall>s. (s \<Turnstile> hml_conj I J \<Phi>) = (s \<Turnstile> (hml_conj I J \<Phi>)))"
+      using neg_case 
+      by (simp add: f_trace_conj)
+    then show ?thesis by blast
+  next
+    assume "\<exists>i\<in>\<Phi> ` I.
+       \<Phi> ` I = {i} \<and> hml_failure_trace i \<and> (\<exists>\<psi>. HML_failure_trace \<psi> \<and> (\<forall>s. (s \<Turnstile> i) = (s \<Turnstile> \<psi>)))"
+    then obtain i \<psi> where IH: "i\<in>\<Phi> ` I" "\<Phi> ` I = {i}" "hml_failure_trace i" "HML_failure_trace \<psi>" "(\<forall>s. (s \<Turnstile> i) = (s \<Turnstile> \<psi>))"
+      by blast
+    then show ?case
+    proof(cases "I \<inter> J = {}")
+      case True
+      define \<Psi> where  \<Psi>_def: "\<Psi> = (\<lambda>x. if x \<in> I then \<psi> else (if x \<in> J then \<Phi> x else undefined))"
+      have "\<Psi> ` I = {\<psi>}" unfolding \<Psi>_def using \<open>\<Phi> ` I = {i}\<close> by auto
+      hence pos: "(\<exists>\<psi> \<in> (\<Psi> ` I). (HML_failure_trace \<psi>) \<and> (\<forall>y \<in> (\<Psi> ` I). \<psi> \<noteq> y \<longrightarrow> nested_empty_conj y))"
+        by (simp add: \<open>HML_failure_trace \<psi>\<close>)
+      hence "\<forall>\<psi> \<in> \<Psi> ` J. stacked_pos_conj_pos \<psi>"
+        unfolding \<Psi>_def
+        using neg_case \<open>I \<inter> J = {}\<close> 
+        by auto
+      hence "HML_failure_trace (hml_conj I J \<Psi>)" using pos 
+        by (simp add: f_trace_conj)
+      from \<Psi>_def have "(\<forall>s. \<forall>j \<in> J. (\<not>(s \<Turnstile> (\<Psi> j)) = (\<not>(s \<Turnstile> (\<Phi> j)))))" using IH 
+        using True by auto
+      from \<Psi>_def have "(\<forall>s. \<forall>i \<in> I. (\<not>(s \<Turnstile> (\<Psi> i)) = (\<not>(s \<Turnstile> (\<Phi> i)))))" using IH 
+        by (metis emptyE imageI insertE)
+      have "(\<forall>s. (s \<Turnstile> hml_conj I J \<Phi>) = (s \<Turnstile> (hml_conj I J \<Psi>)))" using IH hml_sem_conj \<Psi>_def 
+        using \<open>\<forall>s. \<forall>i\<in>I. (s \<Turnstile> \<Psi> i) \<noteq> (\<not> s \<Turnstile> \<Phi> i)\<close> by auto
+    then show ?thesis using \<open>HML_failure_trace (hml_conj I J \<Psi>)\<close> by blast
+    next
+      case False
+      then obtain j where "j \<in> I \<inter> J" by blast
+      from False have "(\<forall>s. \<not>(s \<Turnstile> hml_conj I J \<Phi>))"
+        using index_sets_conj_disjunct 
+        by presburger
+      define \<Psi> where "\<Psi> = (\<lambda>x. if x \<in> (I \<inter> J) then TT::('a, 's) hml else undefined)"
+      with \<open>j \<in> I \<inter> J\<close> have "\<Psi> ` (I \<inter> J) = {TT}" 
+        by auto
+      have "stacked_pos_conj_pos TT" 
+        using stacked_pos_conj_pos.intros(1) by blast
+      hence "(\<forall>y \<in> (\<Psi> ` (I \<inter> J)). stacked_pos_conj_pos y)" using \<Psi>_def \<open>j \<in> I \<inter> J\<close> 
+        using \<open>\<Psi> ` (I \<inter> J) = {TT}\<close> by fastforce
+      have "(\<forall>y \<in> (\<Psi> ` {}). nested_empty_conj y) \<and> (\<forall>y \<in> (\<Psi> ` (I \<inter> J)). stacked_pos_conj_pos y)" 
+        using neg_case 
+        using \<open>\<forall>y\<in>\<Psi> ` (I \<inter> J). stacked_pos_conj_pos y\<close> by blast
+      hence f_trace: "((\<exists>\<psi>\<in>(\<Psi> ` ({}::'s set)). HML_failure_trace \<psi> \<and> (\<forall>y\<in>(\<Psi> ` ({}::'s set)). \<psi> \<noteq> y \<longrightarrow> nested_empty_conj y)) \<or>
+     (\<forall>y\<in>(\<Psi> ` ({}::'s set)). nested_empty_conj y)) \<and>
+    (\<forall>y\<in>(\<Psi> ` (I \<inter> J)). stacked_pos_conj_pos y)" 
+        by fastforce 
+      define \<psi> where "\<psi> \<equiv> (hml_conj ({}::'s set) (I \<inter> J) \<Psi>)"
+      have "HML_failure_trace \<psi>" unfolding \<psi>_def using f_trace_conj f_trace 
+        by fastforce
+      have "\<forall>s. \<not> s \<Turnstile> \<psi>" 
+        using \<Psi>_def \<open>j \<in> I \<inter> J\<close> \<psi>_def by auto
+      then show ?thesis using \<open>HML_failure_trace \<psi>\<close> 
+        using \<open>\<forall>s. \<not> s \<Turnstile> hml_conj I J \<Phi>\<close> by blast
+    qed
+  qed
+qed
+
+lemma stacked_pos_rewriting:
+  assumes "stacked_pos_conj_pos \<phi>" "\<not>HML_true \<phi>"
+  shows "\<exists>\<alpha>. (\<forall>s. (s \<Turnstile> \<phi>) \<longleftrightarrow> (s \<Turnstile> (hml_pos \<alpha> TT)))"
+  using assms proof(induction \<phi>)
+  case 1
+  then show ?case 
+    unfolding HML_true_def
+    using TT_like.intros(1) HML_true_TT_like by simp
+next
+  case (2 \<psi> uu)
+  then show ?case 
+    using HML_true_def HML_true_nested_empty_pos_conj by auto
+next
+  case (3 \<Phi> I J)
+  have "(\<forall>\<psi>\<in>\<Phi> ` I. nested_empty_pos_conj \<psi> \<longrightarrow> HML_true \<psi>)" 
+    using lts.HML_true_nested_empty_pos_conj by blast
+  have "((\<forall>\<psi>\<in>\<Phi> ` I. nested_empty_pos_conj \<psi>) \<and> \<Phi> ` J = {}) \<longrightarrow> HML_true (hml_conj I J \<Phi>)"
+    by (simp add: lts.HML_true_nested_empty_pos_conj nested_empty_pos_conj.intros(2))
+  with 3 obtain \<phi> where "\<phi>\<in>\<Phi> ` I"
+        "stacked_pos_conj_pos \<phi>" "(\<not> HML_true \<phi> \<longrightarrow> (\<exists>\<alpha>. \<forall>s. (s \<Turnstile> \<phi>) = (s \<Turnstile> hml_pos \<alpha> TT)))"
+        "(\<forall>\<psi>\<in>\<Phi> ` I. \<psi> \<noteq> \<phi> \<longrightarrow> nested_empty_pos_conj \<psi>)"
+    by meson
+  then have "\<not> HML_true \<phi>" using 3(3) \<open>(\<forall>\<psi>\<in>\<Phi> ` I. nested_empty_pos_conj \<psi> \<longrightarrow> HML_true \<psi>)\<close>
+    by (smt (verit, ccfv_threshold) "3.hyps" HML_true_def ball_imageD empty_iff empty_is_image hml_sem_conj)
+  then obtain \<alpha> where "\<forall>s. (s \<Turnstile> \<phi>) = (s \<Turnstile> hml_pos \<alpha> TT)" 
+    using \<open>\<not> HML_true \<phi> \<longrightarrow> (\<exists>\<alpha>. \<forall>s. (s \<Turnstile> \<phi>) = (s \<Turnstile> hml_pos \<alpha> TT))\<close> by blast
+  have "\<forall>s. (s \<Turnstile> hml_conj I J \<Phi>) = (s \<Turnstile> hml_pos \<alpha> TT)" 
+    using "3.hyps" "3.prems" HML_true_def \<open>\<forall>\<psi>\<in>\<Phi> ` I. \<psi> \<noteq> \<phi> \<longrightarrow> nested_empty_pos_conj \<psi>\<close> \<open>\<forall>\<psi>\<in>\<Phi> ` I. nested_empty_pos_conj \<psi> \<longrightarrow> HML_true \<psi>\<close> \<open>\<forall>s. (s \<Turnstile> \<phi>) = (s \<Turnstile> hml_pos \<alpha> TT)\<close> by fastforce
+  then show ?case by blast
+qed
+
+lemma nested_empty_conj_TT_or_FF:
+  assumes "nested_empty_conj \<phi>"
+  shows "(\<forall>s. (s \<Turnstile> \<phi>)) \<or> (\<forall>s. \<not>(s \<Turnstile> \<phi>))"
+  using assms HML_true_nested_empty_pos_conj
+  unfolding HML_true_def
+  by(induction, simp, fastforce)
+
+lemma 
+  fixes \<phi> :: "('a, 's) hml"
+  assumes "HML_failure_trace \<phi>"
+  shows "\<exists>\<psi>. hml_failure_trace \<psi> \<and> (\<forall>s. (s \<Turnstile> \<phi>) \<longleftrightarrow> (s \<Turnstile> \<psi>))"
+  using assms proof(induct)
+  case f_trace_tt
+  then show ?case 
+    using hml_failure_trace.intros(1) by blast
+next
+  case (f_trace_pos \<phi> \<alpha>)
+  then obtain \<psi> where "hml_failure_trace \<psi>" "(\<forall>s. (s \<Turnstile> \<phi>) = (s \<Turnstile> \<psi>))" by blast
+  have "hml_failure_trace (hml_pos \<alpha> \<psi>)" 
+    using \<open>hml_failure_trace \<psi>\<close> hml_failure_trace.simps by blast
+  have "(\<forall>s. (s \<Turnstile> hml_pos \<alpha> \<phi>) = (s \<Turnstile> (hml_pos \<alpha> \<psi>)))" 
+    by (simp add: \<open>\<forall>s. (s \<Turnstile> \<phi>) = (s \<Turnstile> \<psi>)\<close>)
+  then show ?case 
+    using \<open>hml_failure_trace (hml_pos \<alpha> \<psi>)\<close> by blast
+next
+  case (f_trace_conj \<Phi> I J)
+  hence neg_case: "\<forall>j\<in>\<Phi> ` J. stacked_pos_conj_pos j" 
+    using stacked_pos_conj_pos.simps nested_empty_pos_conj.intros(1) by auto
+  from f_trace_conj have IH: "((\<exists>\<psi>\<in>\<Phi> ` I.
+            (HML_failure_trace \<psi> \<and> (\<exists>\<psi>'. hml_failure_trace \<psi>' \<and> (\<forall>s. (s \<Turnstile> \<psi>) = (s \<Turnstile> \<psi>')))) \<and>
+            (\<forall>y\<in>\<Phi> ` I. \<psi> \<noteq> y \<longrightarrow> nested_empty_conj y)) \<or>
+        (\<forall>y\<in>\<Phi> ` I. nested_empty_conj y))" 
+    by blast
+  from IH show ?case proof(rule disjE)
+    assume "\<exists>\<psi>\<in>\<Phi> ` I.
+       (HML_failure_trace \<psi> \<and> (\<exists>\<psi>'. hml_failure_trace \<psi>' \<and> (\<forall>s. (s \<Turnstile> \<psi>) = (s \<Turnstile> \<psi>')))) \<and>
+       (\<forall>y\<in>\<Phi> ` I. \<psi> \<noteq> y \<longrightarrow> nested_empty_conj y)"
+    then obtain \<phi> \<psi> where "\<phi>\<in>\<Phi> ` I" "HML_failure_trace \<phi>" "hml_failure_trace \<psi>" 
+                          "(\<forall>s. (s \<Turnstile> \<phi>) = (s \<Turnstile> \<psi>))" "(\<forall>y\<in>\<Phi> ` I. \<phi> \<noteq> y \<longrightarrow> nested_empty_conj y)"
+      by meson
+    then obtain i_\<phi> where "\<Phi> i_\<phi> = \<phi>" 
+      by blast
+    consider "\<exists>y \<in> \<Phi>`I. \<phi> \<noteq> y \<and> (\<forall>s. \<not>(s \<Turnstile> y))" | "(\<forall>y\<in>\<Phi> ` I. \<phi> \<noteq> y \<longrightarrow> HML_true y)"
+      unfolding HML_true_def
+      using nested_empty_conj_TT_or_FF
+      using \<open>\<forall>y\<in>\<Phi> ` I. \<phi> \<noteq> y \<longrightarrow> nested_empty_conj y\<close> by blast
+    then show "\<exists>\<psi>. hml_failure_trace \<psi> \<and> (\<forall>s. (s \<Turnstile> hml_conj I J \<Phi>) = (s \<Turnstile> \<psi>))"
+    proof(cases)
+      case 1
+      hence "\<forall>s. \<not>s \<Turnstile> (hml_conj I J \<Phi>)"
+        using hml_sem_conj by blast
+      obtain y where "y \<in> \<Phi>`I" "\<phi> \<noteq> y \<and> (\<forall>s. \<not> s \<Turnstile> y)" 
+        using "1" by blast
+      define \<Psi> where \<Psi>_def: "\<Psi> = (\<lambda>i. (if i \<in> I then (TT::('a, 's)hml) else undefined))"
+      hence "\<forall>s. \<not>s \<Turnstile> (hml_conj {} I \<Psi>)" 
+        using \<open>y \<in> \<Phi> ` I\<close> by auto
+      have "\<Psi> ` {} = {}" "\<forall>j \<in> \<Psi> ` I. j = TT" 
+         apply blast
+        unfolding \<Psi>_def 
+        using \<open>y \<in> \<Phi>`I\<close> 
+        by simp
+      hence "hml_failure_trace (hml_conj {} I \<Psi>)" 
+        by (meson hml_failure_trace.intros(3))
+      then show ?thesis using \<open>\<forall>s. \<not>s \<Turnstile> (hml_conj I J \<Phi>)\<close> 
+        using \<open>\<forall>s. \<not> s \<Turnstile> hml_conj {} I \<Psi>\<close> by blast
+    next
+      case 2
+      consider "\<forall>y \<in> \<Phi>`J. \<exists>\<alpha>. (\<forall>s. (s \<Turnstile> y) \<longleftrightarrow> (s \<Turnstile> (hml_pos \<alpha> TT)))" | "(\<exists>y\<in>\<Phi> ` J. HML_true y)"
+        unfolding HML_true_def
+        using stacked_pos_rewriting neg_case
+        using that(2) by blast
+      then show ?thesis proof(cases)
+        case 1
+        show ?thesis proof(cases "\<Phi> ` I \<inter> \<Phi> ` J = {}")
+          case True
+          hence "I \<inter> J = {}"
+            by blast
+          from 2 have "\<forall>y\<in>\<Phi> ` I. \<phi> \<noteq> y \<longrightarrow> (\<forall>s. s \<Turnstile> y)"
+            unfolding HML_true_def 
+            by blast
+          hence "\<forall>s. (\<forall>i \<in> I. s \<Turnstile> (\<Phi> i)) \<longleftrightarrow> s \<Turnstile> \<phi>"
+            using \<open>\<phi> \<in> \<Phi> ` I\<close> by auto
+          define \<Psi> where "\<Psi> \<equiv> (\<lambda>i. (if i = i_\<phi> then \<psi> 
+                                    else (if i \<in> J then (hml_pos (SOME \<alpha>. (\<forall>s. (s \<Turnstile> \<Phi> i) \<longleftrightarrow> (s \<Turnstile> (hml_pos \<alpha> TT)))) TT)  
+                                                else undefined)))"
+          have "\<phi> \<notin> \<Phi> ` J"
+            using True \<open>\<phi> \<in> \<Phi> ` I\<close> 
+            by blast
+          hence "\<forall>i \<in> J. \<Psi> i = (hml_pos (SOME \<alpha>. (\<forall>s. (s \<Turnstile> \<Phi> i) \<longleftrightarrow> (s \<Turnstile> (hml_pos \<alpha> TT)))) TT)"
+            using True "1" \<Psi>_def  
+            using \<open>\<Phi> i_\<phi> = \<phi>\<close> by auto
+          have "\<forall>j \<in> J. \<exists>\<alpha>. (\<forall>s. (s \<Turnstile> \<Phi> j) \<longleftrightarrow> (s \<Turnstile> (hml_pos \<alpha> TT)))"
+            using neg_case stacked_pos_rewriting "1" by blast
+          hence "\<forall>j \<in> J. (\<forall>s. (s \<Turnstile> \<Phi> j) \<longleftrightarrow> (s \<Turnstile> \<Psi> j))"
+            using True \<open>\<forall>i \<in> J. \<Psi> i = (hml_pos (SOME \<alpha>. (\<forall>s. (s \<Turnstile> \<Phi> i) \<longleftrightarrow> (s \<Turnstile> (hml_pos \<alpha> TT)))) TT)\<close>
+            by (smt (verit, ccfv_threshold) tfl_some)
+          have "\<forall>i \<in> I. \<Phi> i \<noteq> \<phi> \<longrightarrow> (\<forall>s. s \<Turnstile> \<Phi> i)"
+            by (simp add: \<open>\<forall>y\<in>\<Phi> ` I. \<phi> \<noteq> y \<longrightarrow> (\<forall>s. s \<Turnstile> y)\<close>) 
+          have "\<Psi> ` {i_\<phi>} = {\<psi>}" 
+            using \<Psi>_def \<open>\<phi>\<in>\<Phi> ` I\<close> \<open>\<phi> \<notin> \<Phi> ` J\<close> \<open>I \<inter> J = {}\<close>
+            by simp
+          hence "\<forall>s. (\<forall>i \<in> {i_\<phi>}. s \<Turnstile> (\<Psi> i)) \<longleftrightarrow> s \<Turnstile> \<psi>" 
+            using \<open>\<phi> \<in> \<Phi> ` I\<close> \<Psi>_def \<open>\<Phi> i_\<phi> = \<phi>\<close> by auto
+          hence "\<forall>s. s \<Turnstile> (hml_conj I J \<Phi>) \<longleftrightarrow> s \<Turnstile> (hml_conj {i_\<phi>} J \<Psi>)"
+            using \<open>\<forall>j \<in> J. (\<forall>s. (s \<Turnstile> \<Phi> j) \<longleftrightarrow> (s \<Turnstile> \<Psi> j))\<close>
+            by (simp add: \<open>\<forall>s. (\<forall>i\<in>I. s \<Turnstile> \<Phi> i) = (s \<Turnstile> \<phi>)\<close> \<open>\<forall>s. (s \<Turnstile> \<phi>) = (s \<Turnstile> \<psi>)\<close>)
+          have "\<forall>j \<in> \<Psi> ` J. \<exists>\<alpha>. j = (hml_pos \<alpha> TT)" 
+            using \<open>\<forall>i\<in>J. \<Psi> i = hml_pos (SOME \<alpha>. \<forall>s. (s \<Turnstile> \<Phi> i) = (s \<Turnstile> hml_pos \<alpha> TT)) TT\<close> by blast
+          have "(\<exists>i \<in> \<Psi> ` {i_\<phi>}. \<Psi> ` {i_\<phi>} = {i} \<and> hml_failure_trace i)"
+            using \<Psi>_def
+            using \<open>\<Psi> ` {i_\<phi>} = {\<psi>}\<close> \<open>hml_failure_trace \<psi>\<close> by auto
+          have "hml_failure_trace (hml_conj {i_\<phi>} J \<Psi>)"
+            by (meson \<open>\<exists>i\<in>\<Psi> ` {i_\<phi>}. \<Psi> ` {i_\<phi>} = {i} \<and> hml_failure_trace i\<close> \<open>\<forall>j\<in>\<Psi> ` J. \<exists>\<alpha>. j = hml_pos \<alpha> TT\<close> hml_failure_trace.intros(3))
+          then show ?thesis using \<open>\<forall>s. s \<Turnstile> (hml_conj I J \<Phi>) \<longleftrightarrow> s \<Turnstile> (hml_conj {i_\<phi>} J \<Psi>)\<close>
+            by blast
+        next
+          case False
+          hence "\<forall>s. \<not>(s \<Turnstile> hml_conj I J \<Phi>)" 
+            by fastforce
+          then obtain \<phi> i_\<phi> where "\<phi> \<in> \<Phi> ` I \<inter> \<Phi> ` J" "\<Phi> i_\<phi> = \<phi>" 
+            using False by blast
+          define \<Psi> where "\<Psi> \<equiv> (\<lambda>i. (if i = i_\<phi> then TT::('a, 's)hml else undefined))"
+          hence "\<forall>s. \<not>(s \<Turnstile> hml_conj {} {i_\<phi>} \<Psi>)" 
+            by simp
+          have "hml_failure_trace (hml_conj {} {i_\<phi>} \<Psi>)" 
+            by (simp add: \<Psi>_def hml_failure_trace.intros(3))
+          then show ?thesis using \<open>\<forall>s. \<not>(s \<Turnstile> hml_conj {} {i_\<phi>} \<Psi>)\<close> \<open>\<forall>s. \<not>(s \<Turnstile> hml_conj I J \<Phi>)\<close> 
+            by blast
+        qed
+      next
+        case 2
+        hence "\<forall>s. \<not>s \<Turnstile> (hml_conj I J \<Phi>)" 
+          unfolding HML_true_def 
+          by fastforce
+        obtain y where "y \<in> \<Phi>`J" "(\<forall>s. s \<Turnstile> y)" 
+          using "2"
+          unfolding HML_true_def 
+          by blast
+      define \<Psi> where \<Psi>_def: "\<Psi> = (\<lambda>i. (if i \<in> J then (TT::('a, 's)hml) else undefined))"
+      hence "\<forall>s. \<not>s \<Turnstile> (hml_conj {} J \<Psi>)" 
+        using \<open>y \<in> \<Phi> ` J\<close> by auto
+      have "\<Psi> ` {} = {}" "\<forall>j \<in> \<Psi> ` J. j = TT" 
+         apply blast
+        unfolding \<Psi>_def 
+        using \<open>y \<in> \<Phi>`J\<close> 
+        by simp
+      hence "hml_failure_trace (hml_conj {} J \<Psi>)" 
+        by (meson hml_failure_trace.intros(3))
+      then show ?thesis using \<open>\<forall>s. \<not>s \<Turnstile> (hml_conj I J \<Phi>)\<close> 
+        using \<open>\<forall>s. \<not> s \<Turnstile> hml_conj {} J \<Psi>\<close> by blast
+    qed
+  qed
+next
+    assume "\<forall>y\<in>\<Phi> ` I. nested_empty_conj y"
+    then show ?thesis proof(cases "\<exists>i\<in>I. (\<forall>s. (\<not>(s \<Turnstile> (\<Phi> i))))")
+      case True
+      hence "\<forall>s. (\<not>(s \<Turnstile> hml_conj I J \<Phi>))" 
+        using hml_sem_conj by blast
+      define \<Psi> where "\<Psi> \<equiv> (\<lambda>i. (if i \<in> I then TT:: ('a, 's) hml else undefined))"
+      have "\<forall>j \<in> \<Psi> ` I. j = TT" 
+        using \<Psi>_def by force
+      hence "hml_failure_trace (hml_conj {} I \<Psi>)" using hml_failure_trace.intros(3)
+        by (metis image_empty)
+      have "\<forall>s. (\<not>(s \<Turnstile> hml_conj {} I \<Psi>))" 
+        using True \<Psi>_def by force
+      then show ?thesis using \<open>hml_failure_trace (hml_conj {} I \<Psi>)\<close> \<open>\<forall>s. (\<not>(s \<Turnstile> hml_conj I J \<Phi>))\<close>
+        by blast
+    next
+      case False
+      consider "\<forall>y \<in> \<Phi>`J. \<exists>\<alpha>. (\<forall>s. (s \<Turnstile> y) \<longleftrightarrow> (s \<Turnstile> (hml_pos \<alpha> TT)))" | "(\<exists>y\<in>\<Phi> ` J. HML_true y)"
+        using neg_case stacked_pos_rewriting by blast
+      then show ?thesis proof(cases)
+        case 1
+        from False have "\<forall>i \<in> I. (\<forall>s. (s \<Turnstile> (\<Phi> i)))"
+        using nested_empty_conj_TT_or_FF \<open>\<forall>y\<in>\<Phi> ` I. nested_empty_conj y\<close> by blast 
+        have "\<forall>i \<in> {}. (\<forall>s. (s \<Turnstile> (\<Phi> i)))" by blast
+        define \<Psi> where "\<Psi> \<equiv> (\<lambda>i. (if i \<in> J 
+              then (hml_pos (SOME \<alpha>. (\<forall>s. (s \<Turnstile> (\<Phi> i)) \<longleftrightarrow> (s \<Turnstile> (hml_pos \<alpha> TT)))) TT:: ('a, 's) hml) 
+              else undefined))"
+      have "\<forall>j\<in>\<Phi> ` J. (\<exists>\<alpha>. (\<forall>s. (s \<Turnstile> j) \<longleftrightarrow> (s \<Turnstile> (hml_pos \<alpha> TT))))" 
+        using stacked_pos_rewriting neg_case 1 by blast
+      hence "\<forall>j \<in> J. (\<exists>\<alpha>. (\<forall>s. (s \<Turnstile> \<Phi> j) \<longleftrightarrow> (s \<Turnstile> (hml_pos \<alpha> TT))))" 
+        by blast
+      hence "\<forall>j \<in> J. \<exists>\<alpha> .\<Psi> j = (hml_pos \<alpha> TT) \<and> (\<forall>s. (s \<Turnstile> (\<Phi> j)) \<longleftrightarrow> (s \<Turnstile> (hml_pos \<alpha> TT)))"
+      proof(safe)
+        fix j
+        assume "\<forall>j\<in>J. \<exists>\<alpha>. \<forall>s. (s \<Turnstile> \<Phi> j) = (s \<Turnstile> hml_pos \<alpha> TT)" "j \<in> J"
+        then obtain \<alpha> where "\<Psi> j = hml_pos \<alpha> TT" 
+          using \<Psi>_def by fastforce
+        hence "(\<forall>s. (s \<Turnstile> (\<Phi> j)) \<longleftrightarrow> (s \<Turnstile> (hml_pos \<alpha> TT)))" unfolding \<Psi>_def using \<open>j \<in> J\<close> 
+          by (smt (verit, best) \<open>\<forall>j\<in>J. \<exists>\<alpha>. \<forall>s. (s \<Turnstile> \<Phi> j) = (s \<Turnstile> hml_pos \<alpha> TT)\<close> tfl_some)
+        then show "\<exists>\<alpha>. \<Psi> j = hml_pos \<alpha> TT \<and> (\<forall>s. (s \<Turnstile> \<Phi> j) = (s \<Turnstile> hml_pos \<alpha> TT))"
+          using \<open>\<Psi> j = hml_pos \<alpha> TT\<close> by blast
+      qed
+      hence "\<forall>j \<in> J. \<forall>s. s \<Turnstile> (\<Psi> j) \<longleftrightarrow> s \<Turnstile> (\<Phi> j)" using \<Psi>_def 
+        by metis
+      hence "\<forall>j \<in> J. \<forall>s. \<not>s \<Turnstile> (\<Psi> j) \<longleftrightarrow> \<not>s \<Turnstile> (\<Phi> j)" by blast
+      hence "(\<forall>s. (s \<Turnstile> hml_conj I J \<Phi>) = (s \<Turnstile> hml_conj {} J \<Psi>))"
+        using \<open>\<forall>i \<in> I. (\<forall>s. (s \<Turnstile> (\<Phi> i)))\<close> \<open>\<forall>i \<in> {}. (\<forall>s. (s \<Turnstile> (\<Phi> i)))\<close> 
+        by simp
+      have "\<forall>j \<in> \<Psi> ` J. \<exists>\<alpha>. j = (hml_pos \<alpha> TT)" 
+        by (simp add: \<Psi>_def)
+      hence "hml_failure_trace (hml_conj {} J \<Psi>)" 
+        by (simp add: hml_failure_trace.intros(3))
+      then show ?thesis
+        using \<open>\<forall>s. (s \<Turnstile> hml_conj I J \<Phi>) = (s \<Turnstile> hml_conj {} J \<Psi>)\<close> by blast
+      next
+        case 2
+        hence "\<forall>s. \<not>s \<Turnstile> (hml_conj I J \<Phi>)" 
+          unfolding HML_true_def 
+          by fastforce
+        obtain y where "y \<in> \<Phi>`J" "(\<forall>s. s \<Turnstile> y)" 
+          using "2"
+          unfolding HML_true_def 
+          by blast
+        define \<Psi> where \<Psi>_def: "\<Psi> = (\<lambda>i. (if i \<in> J then (TT::('a, 's)hml) else undefined))"
+        hence "\<forall>s. \<not>s \<Turnstile> (hml_conj {} J \<Psi>)" 
+          using \<open>y \<in> \<Phi> ` J\<close> by auto
+        have "\<Psi> ` {} = {}" "\<forall>j \<in> \<Psi> ` J. j = TT" 
+           apply blast
+          unfolding \<Psi>_def 
+          using \<open>y \<in> \<Phi>`J\<close> 
+          by simp
+        hence "hml_failure_trace (hml_conj {} J \<Psi>)" 
+          by (meson hml_failure_trace.intros(3))
+        then show ?thesis using \<open>\<forall>s. \<not>s \<Turnstile> (hml_conj I J \<Phi>)\<close> 
+          using \<open>\<forall>s. \<not> s \<Turnstile> hml_conj {} J \<Psi>\<close> by blast
+      qed
+    qed
+  qed 
+qed
+
+end
+end
