Relational_Equivalences.thy
@@ -1,0 +1,137 @@
+(*<*)
+theory Relational_Equivalences
+  imports Main
+"HOL-Library.Countable_Set"
+Transition_Systems
+begin
+(*>*)
+
+context lts
+begin
+text \<open>Introduce these definitions later?\<close>
+
+abbreviation traces :: \<open>'s \<Rightarrow> 'a list set\<close> where
+\<open>traces p \<equiv> {tr. \<exists>p'. p \<mapsto>$ tr p'}\<close>
+
+abbreviation all_traces :: "'a list set" where
+"all_traces \<equiv>{tr. \<exists>p p'. p \<mapsto>$ tr p'}"
+
+inductive paths:: \<open>'s \<Rightarrow> 's list \<Rightarrow> 's \<Rightarrow> bool\<close> where
+\<open>paths p [] p\<close> |
+\<open>paths p (a#as) p''\<close> if "\<exists>\<alpha>. p \<mapsto> \<alpha> a \<and> (paths a as p'')"
+
+lemma path_implies_seq:
+  assumes A1: "\<exists>xs. paths p xs p'"
+  shows "\<exists>ys. p \<mapsto>$ ys p'"
+proof-
+  from A1 obtain xs where "paths p xs p'" by auto
+  then show "\<exists>ys. p \<mapsto>$ ys p'"
+proof (rule local.paths.induct)
+  fix q
+  have "q \<mapsto>$ [] q" using step_sequence.intros(1).
+  then show "\<exists>ys. q \<mapsto>$ ys q" by (rule exI)
+next
+  fix p a as p''
+  assume A1: "\<exists>\<alpha>. p \<mapsto>\<alpha> a \<and> paths a as p'' \<and> (\<exists>ys. a \<mapsto>$ ys p'')"
+  then obtain ys \<alpha> where A2: "a \<mapsto>$ ys p''" and A3: "p \<mapsto>\<alpha> a"
+    by blast
+  then have "p \<mapsto>$ (\<alpha>#ys) p''" using step_sequence.intros(2)
+    by blast
+  then show "\<exists>ys. p \<mapsto>$ ys p''" by (rule exI)
+  qed
+qed
+
+lemma seq_implies_path:
+  assumes A1: "\<exists>ys. p \<mapsto>$ ys p'"
+  shows "\<exists>xs. paths p xs p'"
+proof-
+  from A1 obtain ys where "p \<mapsto>$ ys p'" by auto
+  then show "\<exists>xs. paths p xs p'"
+  proof(rule step_sequence.induct)
+    fix p
+    have "paths p [] p" using paths.intros(1).
+    then show "\<exists>xs. paths p xs p" by (rule exI)
+  next
+    fix p a rt p''
+    assume "\<exists>p'. p \<mapsto>a p' \<and> p' \<mapsto>$ rt p'' \<and> (\<exists>xs. paths p' xs p'')"
+    then obtain p' xs where "p \<mapsto>a p'" and "paths p' xs p''" by auto
+    then have "paths p (p'#xs) p''" using paths.intros(2) by blast
+    then show "\<exists>xs. paths p xs p''" by (rule exI)
+  qed
+qed
+
+text \<open>Trace preorder as inclusion of trace sets\<close>
+
+definition trace_preordered (infix \<open>\<lesssim>T\<close> 60)where
+\<open>trace_preordered p q \<equiv> traces p \<subseteq> traces q\<close>
+
+text \<open>Trace equivalence as mutual preorder\<close>
+
+abbreviation trace_equivalent (infix \<open>\<simeq>T\<close> 60) where
+\<open>p \<simeq>T q \<equiv> p \<lesssim>T q \<and> q \<lesssim>T p\<close>
+
+text \<open>Trace preorder is transitive\<close>
+
+lemma T_trans:
+  shows \<open>transp (\<lesssim>T)\<close>
+  unfolding transp_def trace_preordered_def by blast
+
+text \<open>Failure Pairs\<close>
+
+abbreviation failure_pairs :: \<open>'s \<Rightarrow> ('a list \<times> 'a set) set\<close>
+  where
+\<open>failure_pairs p \<equiv> {(xs, F)|xs F. \<exists>p'. p \<mapsto>$ xs p' \<and> (initial_actions p' \<inter> F = {})}\<close>
+
+text \<open>Failure preorder and -equivalence\<close>
+
+definition failure_preordered (infix \<open>\<lesssim>F\<close> 60) where
+\<open>p \<lesssim>F q \<equiv> failure_pairs p \<subseteq> failure_pairs q\<close>
+
+abbreviation failure_equivalent (infix \<open>\<simeq>F\<close> 60) where
+\<open> p \<simeq>F q \<equiv> p \<lesssim>F q \<and> q \<lesssim>F p\<close>
+
+text \<open>Possible future sets\<close>
+
+abbreviation possible_future_pairs :: \<open>'s \<Rightarrow> ('a list \<times> 'a list list) set\<close>
+  where
+\<open>possible_future_pairs p \<equiv> {(xs, X)|xs X. \<exists>p'. p \<mapsto>$ xs p' \<and> traces p' = (set X)}\<close>
+
+definition possible_futures_equivalent (infix \<open>\<simeq>PF\<close> 60) where
+\<open>p \<simeq>PF q \<equiv> (possible_future_pairs p = possible_future_pairs q)\<close>
+
+lemma PF_trans: "transp (\<simeq>PF)"
+  unfolding possible_futures_equivalent_def
+  by (simp add: transp_def)
+
+text \<open>isomorphism\<close>
+
+definition isomorphism :: \<open>('s \<Rightarrow> 's) \<Rightarrow> bool\<close> where
+\<open>isomorphism f \<equiv> bij f \<and> (\<forall>p a p'. p \<mapsto> a p' \<longleftrightarrow> f p \<mapsto> a (f p'))\<close>
+
+definition is_isomorphic :: \<open>'s \<Rightarrow> 's \<Rightarrow> bool\<close> (infix \<open>\<simeq>ISO\<close> 60) where
+\<open>p \<simeq>ISO q \<equiv> \<exists>f. isomorphism f \<and> (f p) = q\<close>
+
+text \<open>Two states are simulation preordered if they can be related by
+  a simulation relation. (Implied by isometry.)\<close>
+
+definition simulation
+  where \<open>simulation R \<equiv>
+    \<forall>p q a p'. p \<mapsto> a p' \<and> R p q \<longrightarrow> (\<exists>q'. q \<mapsto> a q' \<and> R p' q')\<close>
+
+definition simulated_by (infix \<open>\<lesssim>S\<close> 60)
+  where \<open>p \<lesssim>S q \<equiv> \<exists>R. R p q \<and> simulation R\<close>
+
+text \<open>Two states are bisimilar if they can be related by a symmetric simulation.\<close>
+
+definition bisimilar (infix \<open>\<simeq>B\<close> 80) where
+  \<open>p \<simeq>B q \<equiv> \<exists>R. simulation R \<and> symp R \<and> R p q\<close>
+
+text \<open>Bisimilarity is a simulation.\<close>
+
+lemma bisim_sim:
+  shows \<open>simulation (\<simeq>B)\<close>
+  unfolding bisimilar_def simulation_def by blast
+
+
+end
+end
