ROOT
@@ -9,5 +9,8 @@ sessions
     Introduction
     Foundations
     Transition_Systems
+    Relational_Equivalences
+    HML_list
+    formula_prices_list
   document_files
     "root.tex"
